papers/116_stefan_rass/Supplementary/Misc.thy
@@ -2,6 +2,8 @@ theory Misc
   imports Main
 begin
 
+lemma if_cases: "P a \<Longrightarrow> P b \<Longrightarrow> P (If c a b)" by presburger
+
 lemma inj_imp_inj_on: "inj f \<Longrightarrow> inj_on f A" by (simp add: inj_on_def)
 
 lemma inv_into_onto: "inj_on f A \<Longrightarrow> inv_into A f ` f ` A = A" by simp
